

$$\frac{G(z)}{z} = \frac{32,4z + 3240}{z(z - 2,16)(z + 2,31)} = \frac{A}{z} + \frac{B}{(z - 2,16)} + \frac{C}{(z + 2,31)}$$

$$A = \frac{3240}{(-2,16) \cdot (2,31)} = -649,3506$$

$$B = \frac{32,4 \cdot 2,16 + 3240}{2,16(2,16 + 2,31)} = 342,8188$$

$$C = \frac{32,4 \cdot (-2,31) + 3240}{(-2,31)(-2,31 - 2,16)} = 306,5378$$

$$\frac{G(z)}{z} = \frac{-649,3506}{z} + \frac{342,8188}{z - 2,16} + \frac{306,5378}{z + 2,31}$$

$$z \left\{ \frac{G(z)}{z} \right\} = \frac{-649,3506}{1 - z^{-1}} + \frac{342,8188}{1 - e^{2,16T} \cdot z^{-1}} + \frac{306,5378}{1 - e^{-2,31T} \cdot z^{-1}}$$

$$\frac{-649,3506 \cdot (1 - e^{2,16T} \cdot z^{-1}) \cdot (1 - e^{-2,31T} \cdot z^{-1}) + 342,8188 \cdot (1 - e^{-2,31T} \cdot z^{-1}) + 306,5378 \cdot (1 - e^{2,16T} \cdot z^{-1})}{(1 - z^{-1})(1 - e^{2,16T} \cdot z^{-1})(1 - e^{-2,31T} \cdot z^{-1})}$$

$$P(z) = 0,041$$

$$A = (1 - 1,0218 \cdot z^{-1}) \quad C = (1 - z^{-1})$$

$$u.c = 1 - 1,9772 \cdot z^{-1} + 0,9772 \cdot z^{-2}$$

$$u = (1 - 0,9772 \cdot z^{-1})$$

$$u.c = 1 - 1,999 \cdot z^{-1} + 0,9985 \cdot z^{-2}$$

$$G(z) = \frac{-649,3506 + 1228,0518 \cdot z^{-1} - 648,3785 \cdot z^{-2} + 342,8188 - 677,8213 \cdot z^{-1} + 335,0025 \cdot z^{-2}}{1 - 1,999 \cdot z^{-1} + 0,9985 \cdot z^{-2}}$$

remando os 2 primeiros:

$$-306,5318 + 620,2305 \cdot z^{-1} - 313,3760 \cdot z^{-2} + 306,5318 - 618,7460 \cdot z^{-1} + 313,2412 \cdot z^{-2}$$

Final tem:

$$G(z) = \frac{0,4845 \cdot z^{-1} - 0,1618 \cdot z^{-2}}{1 - 1,999 \cdot z^{-1} + 0,9985 \cdot z^{-2}}$$

lm(z)

→ plim de 0,4857 e 0,1618

$$G(z) = \frac{0,4845 \cdot z - 0,1618}{z^2 - 1,999 \cdot z + 0,9985}$$

aparte num

mul
↓

$$0,3227 \cdot z$$

ou

$$0,3238 \cdot z$$

com mais zeros (computacional)

~~com mais zeros~~
↓

→ mais zeros

$$G(z) = \frac{0,4857 \cdot z - 0,1618}{z^2 - 1,999 \cdot z + 0,9985} \quad \text{com} = \frac{0,3238 \cdot z}{z^2 - 1,999 \cdot z + 0,9985}$$

$$\frac{1 \ln(0.3)}{\sqrt{\pi^2 + \ln^2(0.3)}}$$

$$\zeta \approx 0.3578$$

$$\zeta \approx 0.3579$$

$$\frac{4}{0.3578 \cdot 0.3}$$

$$\omega_n > 3.7264$$

$$\omega_n > 3.7265$$

Polar dominant

$$\zeta = 0.5$$

$$\omega_n = 5$$

$$s_{1,2} = -\zeta \omega_n \pm j \omega_n \sqrt{1 - \zeta^2}$$

$$s_{1,2} = -2.5 \pm j 4.3301$$

$$z_{1,2} = e^{-s_{1,2} \cdot T} = e^{-2.5 \cdot 0.01} \cdot e^{\pm j 4.3301 \cdot 0.01}$$

$$z_{1,2} = e^{-0.025} \cdot e^{\pm j 0.0433}$$

$$z_{1,2} = 0.9753$$